scheduler/example/NDSMainAll.v
@@ -8,64 +8,220 @@ Require Import NDSMainI NDSMainA NDSMainIAproof.
 
 Module NDSMainAll.
   Import inv_instances.
+
+  (* mem *)
+  Local Definition csl : string → bool := λ _, false.
+  (* global environment - not used in this example *)
+  Local Definition genv : GEnv.t := [].
+  
   Local Instance Γ : HRA := ##[invΓ; concΓ; newschΓ; rrsΓ; memΓ; nodeΓ].
-  Local Instance Σ : GRA := ##[Γ; invΣ; newschΣ].
-  Local Definition irΓ : Γ := **[ir_invΓ; ir_concΓ].
-  Local Definition irΣ : Σ := **[irΓ; ir_invΣ].
+  Local Instance Σ : GRA := ##[Γ; invΣ; newschΣ; rrsΣ].
+  Local Definition irΓ : Γ :=
+    **[ir_invΓ; ir_concΓ; SchA.ir_schΓ; RRSAS.ir_schΓ; (ir_memΓ csl genv); RRSNodeAS.ir_nodeΓ].
+  Local Definition irΣ : Σ := **[irΓ; ir_invΣ; SchA.ir_schΣ; RRSAS.ir_schΣ].
 
   Local Lemma irΣ_valid : ✓ (irΣ ⋅ ir_own_admin).
   Proof.
     solve_ir_valid.
-    - apply CannonAS.ir_valid.
+    - apply ir_tidRA_valid.
+    - apply ir_yieldRA_valid.
+    - apply SchA.ir_newtidRA_valid.
+    - apply RRSAS.ir_initRA_valid.
+    - apply RRSAS.ir_ctlRA_valid.
+    - apply RRSAS.ir_pubRA_valid.
+    - apply RRSAS.ir_newtidRA_valid.
+    - apply ir_memRA_valid.
+    - apply RRSNodeAS.ir_nodeRA_valid.
+    - apply SchA.ir_joinRA_valid.
+    - apply RRSAS.ir_invRA_valid.
   Qed.
 
-  Local Definition smod_src : SMod.t := CannonA.smod ☆ (MainA.smod 1).
+  Local Definition sp_rrs : spl_type := (RRSNodeAS.sp ⊤) ++ MemA.sp.
+  Local Definition sp_sch : spl_type := NDSMainA.sp ++ (RRSAS.sp sp_rrs ⊤) ++ sp_rrs.
+
+  Local Definition smod_src : SMod.t :=
+    (NDSMainA.smod)
+      ☆ (SchA.smod sp_sch)
+      ☆ (RRSA.smod sp_rrs)
+      ☆ (RRSNodeA.smod ⊤)
+      ☆ (MemA.smod).
   Local Definition mod_top : Mod.t := (SMod.to_mod sp_none (SMod.cancel smod_src)).
-  Local Definition mod_tgt : Mod.t := CannonI.t ★ (MainI.t 1).
+  Local Definition mod_tgt : Mod.t :=
+    NDSMainI.t
+      ★ SchI.t
+      ★ RRSI.t
+      ★ RRSNodeI.t
+      ★ (MemI.t csl genv).
   
   Local Definition sp : sp_type := sp_from smod_src.
   Local Definition mod_src : Mod.t := SMod.to_mod sp smod_src.
 
   Local Definition init_cond : iProp Σ :=
-    winv (⊤, ⊤) ∗ CannonA.init_cond ∗ MainA.init_cond.
+    winv (⊤, ⊤) ∗ SchA.init_cond ∗ NDSMainA.init_cond ∗ RRSA.init_cond ∗ MemA.init_cond csl genv.
 
   (* Apply cancellation to linked spec module *)
   Lemma cancel_src :
-    refines (mod_top, init_cond)
+    refines (mod_top, init_cond ∗ TIDAUTH 0 ∗ YIELDAUTH 1)%I
             (mod_src, init_cond).
   Proof.
-    eapply Cancel.cancellation.
-    - ii; des; subst; inv FIND; ss; rewrite !eq_rel_dec_correct in H0; des_ifs.
-    - econs; [refl|]; i; inv NS; des; inv H; des; inv H1;
-      rewrite !eq_rel_dec_correct in H2; des_ifs.
-    - econs; unfold_mod; ss; prove_nodup.
+    eapply Cancel.cancellation. econs.
+    - inv FIND; rewrite !eq_rel_dec_correct in H0; des_ifs.
+    - inv FIND; rewrite !eq_rel_dec_correct in H0; des_ifs.
   Qed.
+
+  Section SP.
+
+    Lemma sumbool_convert (a b: string) :
+      sumbool_to_bool (dec (Some a) (Some b)) = (decide (a = b)).
+    Proof.
+      rewrite /dec /option_Dec /AList.option_Dec_obligation_1.
+      des_ifs; ss.
+      { destruct (decide (b = b)); ss. }
+      { destruct (decide (a = b)); ss. }
+    Qed.
+
+    Lemma spsch_in_sp : sp_incl sp_sch sp.
+    Proof.
+      rewrite /sp_sch /sp /smod_src.
+      rewrite /NDSMainA.sp /RRSAS.sp /sp_rrs /RRSNodeAS.sp /MemA.sp. unseal CRIS.
+      prove_nodup.
+      i. ss. rewrite /sp_from /to_sp.
+      rewrite /NDSMainA.smod /SchA.smod /RRSA.smod /RRSNodeA.smod /MemA.smod /=.
+      rewrite !sumbool_convert in H. rewrite !sumbool_convert.
+      destruct (decide (fn = RRSHeader.RRSHdr.init)); subst; [by inv H|ss].
+      destruct (decide (fn = RRSHeader.RRSHdr._spawn)); subst; [by inv H|ss].
+      destruct (decide (fn = RRSHeader.RRSHdr.spawn)); subst; [by inv H|ss].
+      destruct (decide (fn = RRSHeader.RRSHdr.yield)); subst; [by inv H|ss].
+      destruct (decide (fn = RRSHeader.RRSHdr.yield_global)); subst; [by inv H|ss].
+      destruct (decide (fn = RRSHeader.RRSHdr.get_tid)); subst; [by inv H|ss].
+      destruct (decide (fn = RRSNodeHeader.RRSNodeHdr.f_main)); subst; [by inv H|ss].
+      destruct (decide (fn = RRSNodeHeader.RRSNodeHdr.f)); subst; [by inv H|ss].
+      destruct (decide (fn = MemHeader.MemHdr.alloc)); subst; [by inv H|ss].
+      destruct (decide (fn = MemHeader.MemHdr.free)); subst; [by inv H|ss].
+      destruct (decide (fn = MemHeader.MemHdr.load)); subst; [by inv H|ss].
+      destruct (decide (fn = MemHeader.MemHdr.cmp)); subst; [by inv H|ss].
+      destruct (decide (fn = MemHeader.MemHdr.cas)); subst; [by inv H|ss].
+      destruct (decide (fn = MemHeader.MemHdr.store)); subst; [by inv H|ss].
+    Qed.
+
+    Lemma sprrs_in_spsch : spl_sub sp_rrs sp_sch.
+    Proof.
+      rewrite /spl_sub /sp_sch /sp_rrs. i.
+      rewrite /RRSNodeAS.sp /MemA.sp /= in H. revert H. unseal CRIS.
+      i; ss. rewrite !eq_rel_dec_correct in H.
+      des_ifs; rewrite /NDSMainA.sp /RRSAS.sp /RRSNodeAS.sp /MemA.sp; unseal CRIS; ss.
+    Qed.
+
+    Lemma sch_in_sp : sp_incl (SchA.sp sp_sch ⊤) sp.
+    Proof.
+      rewrite /sp_incl /sp /SchA.sp /sp_sch /sp_rrs /sp_from /to_sp /smod_src.
+      rewrite /NDSMainA.sp /RRSAS.sp /sp_rrs /RRSNodeAS.sp /MemA.sp /sp_sch. unseal CRIS.
+      prove_nodup. ss. intros fn fsp. rewrite !sumbool_convert. i.
+      destruct (decide (fn = RRSHeader.RRSHdr.init)); subst; [by inv H|ss].
+      destruct (decide (fn = RRSHeader.RRSHdr._spawn)); subst; [by inv H|ss].
+      destruct (decide (fn = RRSHeader.RRSHdr.spawn)); subst; [by inv H|ss].
+      destruct (decide (fn = RRSHeader.RRSHdr.yield)); subst; [by inv H|ss].
+      destruct (decide (fn = RRSHeader.RRSHdr.yield_global)); subst; [by inv H|ss].
+      destruct (decide (fn = RRSHeader.RRSHdr.get_tid)); subst; [by inv H|ss].
+      destruct (decide (fn = RRSNodeHeader.RRSNodeHdr.f_main)); subst; [by inv H|ss].
+      destruct (decide (fn = RRSNodeHeader.RRSNodeHdr.f)); subst; [by inv H|ss].
+      destruct (decide (fn = MemHeader.MemHdr.alloc)); subst; [by inv H|ss].
+      destruct (decide (fn = MemHeader.MemHdr.free)); subst; [by inv H|ss].
+      destruct (decide (fn = MemHeader.MemHdr.load)); subst; [by inv H|ss].
+      destruct (decide (fn = MemHeader.MemHdr.cmp)); subst; [by inv H|ss].
+      destruct (decide (fn = MemHeader.MemHdr.cas)); subst; [by inv H|ss].
+      destruct (decide (fn = MemHeader.MemHdr.store)); subst; [by inv H|ss].
+      rewrite /NDSMainA.sp /RRSAS.sp /sp_rrs /RRSNodeAS.sp /MemA.sp /sp_sch. unseal CRIS.
+      destruct (decide (fn = SchHeader.SchHdr._spawn)); subst; [by inv H|ss].
+      destruct (decide (fn = SchHeader.SchHdr.spawn)); subst; [by inv H|ss].
+      destruct (decide (fn = SchHeader.SchHdr.yield)); subst; [by inv H|ss].
+      destruct (decide (fn = SchHeader.SchHdr.get_tid)); subst; [by inv H|ss].
+      destruct (decide (fn = SchHeader.SchHdr.join)); subst; [by inv H|ss].
+    Qed.
+
+    Lemma rrs_in_spsch : spl_sub (RRSAS.sp sp_rrs ⊤) sp_sch.
+    Proof.
+      rewrite /spl_sub /RRSAS.sp /sp_sch /sp_rrs.
+      rewrite /NDSMainA.sp /SchA.sp /RRSAS.sp /RRSNodeAS.sp /MemA.sp. unseal CRIS.
+      ss. intros fn fsp. rewrite !eq_rel_dec_correct. des_ifs.
+    Qed.
+
+    Lemma node_in_sprrs : spl_sub (RRSNodeAS.sp ⊤) sp_rrs.
+    Proof.
+      rewrite /spl_sub /RRSNodeAS.sp /sp_sch /sp_rrs.
+      rewrite /NDSMainA.sp /SchA.sp /RRSAS.sp /RRSNodeAS.sp /MemA.sp. unseal CRIS.
+      ss. intros fn fsp. rewrite !eq_rel_dec_correct. des_ifs.
+    Qed.
+
+    Lemma rrs_in_sp : sp_incl (RRSAS.sp sp_rrs ⊤) sp.
+    Proof.
+      rewrite /sp_incl /sp /SchA.sp /sp_sch /sp_rrs /sp_from /to_sp /smod_src.
+      rewrite /NDSMainA.sp /RRSAS.sp /sp_rrs /RRSNodeAS.sp /MemA.sp /sp_sch. unseal CRIS.
+      prove_nodup. ss. intros fn fsp. rewrite !sumbool_convert. i.
+      destruct (decide (fn = RRSHeader.RRSHdr.init)); subst; [by inv H|ss].
+      destruct (decide (fn = RRSHeader.RRSHdr._spawn)); subst; [by inv H|ss].
+      destruct (decide (fn = RRSHeader.RRSHdr.spawn)); subst; [by inv H|ss].
+      destruct (decide (fn = RRSHeader.RRSHdr.yield)); subst; [by inv H|ss].
+      destruct (decide (fn = RRSHeader.RRSHdr.yield_global)); subst; [by inv H|ss].
+      destruct (decide (fn = RRSHeader.RRSHdr.get_tid)); subst; [by inv H|ss].
+    Qed.
+
+  End SP.
 
   (* Refinement between spec/impl of whole program (linked module) *)
   Lemma src_tgt : refines (mod_src, init_cond) (mod_tgt, emp%I).
   Proof.
     eapply ctxr_refines.
-    rewrite /mod_src /mod_tgt /smod_src add_interp_comm.
+    rewrite /mod_src /mod_tgt /smod_src !add_interp_comm.
 
     etrans; cycle 1.
-    { ctxr_rotate. ctxr_drop. eapply CannonIA.ctxr. }
-
-    etrans; cycle 1.
-    { ctxr_rotate. ctxr_drop. eapply CannonMainIA.ctxr.
-      instantiate (1:=sp).
-      rewrite /CannonAS.Sp. unseal CRIS. econs; first prove_nodup.
-      ii. inv H. des_ifs.
-      unfold dec, option_Dec, AList.option_Dec_obligation_1 in Heq.
-      des_ifs.
+    { ctxr_rotate. do 4 ctxr_drop. eapply NDSMainIAproof.ctxr.
+      { eapply spsch_in_sp. }
+      { eapply sprrs_in_spsch. }
+      { eapply sch_in_sp. }
+      { eapply rrs_in_spsch. }
+      { eapply node_in_sprrs. }
     }
 
-    rewrite /CannonA.t /MainA.t /init_cond. unseal CRIS. 
+    etrans; cycle 1.
+    { ctxr_rotate. do 4 ctxr_drop. eapply SchIA.ctxr.
+      { eapply sch_in_sp. }
+      { eapply spsch_in_sp. }
+    }
+
+    etrans; cycle 1.
+    { ctxr_rotate. do 4 ctxr_drop. eapply RRSIA.ctxr.
+      { eapply sch_in_sp. }
+      { eapply rrs_in_sp. }
+      { eapply spsch_in_sp. }
+      { eapply sprrs_in_spsch. }
+    }
+
+    etrans; cycle 1.
+    { do 2 ctxr_rotate. do 4 ctxr_drop. eapply MemIA.ctxr. }
+
+    etrans; cycle 1.
+    { do 2 ctxr_drop. ctxr_rotate. eapply RRSNodeIAproof.ctxr; cycle 1.
+      { eapply spsch_in_sp. }
+      { eapply sprrs_in_spsch. }
+      { eapply sch_in_sp. }
+      { eapply rrs_in_spsch. }
+      { eapply node_in_sprrs. }
+      { set_solver. }
+    }
+
+    etrans; cycle 1.
+    { do 2 ctxr_drop. do 2 ctxr_rotate. ctxr_refl. }
+
+    rewrite /init_cond.
+    rewrite /NDSMainA.t /SchA.t /RRSA.t /RRSNodeA.t /MemA.t. unseal CRIS.
+
     eapply ctxr_cond_strengthen.
-    iIntros "[? [? ?]]". iFrame.
-  (*SLOW*)Qed.
+    iIntros "(? & ? & ? & ? & ?)". iFrame.
+  Qed.
 
   Lemma top_tgt :
-    refines (mod_top, init_cond)
+    refines (mod_top, init_cond ∗ TIDAUTH 0 ∗ YIELDAUTH 1)%I
             (mod_tgt, emp%I).
   Proof.
     etrans.
@@ -76,18 +232,35 @@ Module NDSMainAll.
   Lemma tgt_wf:
     Mod.wf mod_tgt.
   Proof.
-    rewrite /mod_tgt /CannonI.t /MainI.t; unseal CRIS; prove_nodup.
+    rewrite /mod_tgt /NDSMainI.t /SchI.t /RRSI.t /RRSNodeI.t /MemI.t.
+    unseal CRIS. prove_nodup.
   Qed.
 
   Lemma init_cond_valid:
-    ∃ rs, ✓ rs ∧ (Own rs ⊢ |==> init_cond).
+    ∃ rs, ✓ rs ∧ (Own rs ⊢ |==> init_cond ∗ TIDAUTH 0 ∗ YIELDAUTH 1).
   Proof.
     exists (irΣ ⋅ ir_own_admin). split.
     - apply irΣ_valid.
     - simplify_res.
       { rewrite make_own_admin; iFrame.
-        iDestruct "H12" as "[? ?]". iFrame. et.
-      }
+        rewrite /RRSAS.ir_invRA /RRSNodeAS.ir_nodeRA /ir_memRA.
+        rewrite /RRSAS.ir_tidRA /RRSAS.ir_pubRA /RRSAS.ir_initRA.
+        rewrite /RRSAS.ir_ctlRA /ir_yieldRA /ir_tidRA.
+        rewrite /NDSMainA.init_cond /RRSA.init_cond /MemA.init_cond.
+        rewrite /RRSAS.InitRRS /RRSNodeAS.full_val /RRSAS.init_inv.
+        rewrite /TidTokenAuth /YieldTokenAuth.
+        rewrite /RRSAS.rrinv /RRSAS.Pending /RRSAS.Control.
+        rewrite /RRSNodeAS.full_val_r /mem_init_auth.
+        rewrite /RRSAS.init_tid /RRSAS.init_pub.
+        iDestruct "H30" as "[? ?]".
+        unseal RRSHeader.RRS. unseal "Node". unseal "Conc".
+        rewrite /RRSAS.rrinv_admin_r /RRSAS.init_invmap /RRSAS.rrinv_r.
+        iFrame. ss.
+        rewrite dom_empty elements_empty /= !right_id.
+        rewrite -{1}Qp.half_half -dfrac_op_own. rewrite fmap_empty.
+        rewrite gmap_view.gmap_view_auth_dfrac_op.
+        iDestruct "H10" as "[? ?]".
+        iFrame. iPureIntro. esplits; ss. }
       all: solve_res.
   Qed.
 
@@ -98,9 +271,9 @@ Module NDSMainAll.
   Proof.
     move: (top_tgt)=>H; rewrite /refines in H; des; ss.
     hexploit H; eauto using tgt_wf. clear H; intros [WF H].
-    assert (IV: init_cond_valid). des.
+    pose proof init_cond_valid as IV. des.
     destruct (H rs); des; et.
-    rewrite IV0 /init_cond {1}winv_split_empty. iIntros ">[[? ?] ?]". iFrame. et.
+    rewrite IV0 /init_cond {1}winv_split_empty. iIntros ">[[[? ?] ?] ?]". iFrame. eauto.
   Qed.
-(*SLOW*)End CannonAll.
-(* Print Assumptions CannonAll.behavioral_refinement. *)
+(*SLOW*)End NDSMainAll.
+(* Print Assumptions NDSMainAll.behavioral_refinement. *)
